Many more theorems about first sets (taken from Aditi Barthwal's PhD)

examples/parsing/NTpropertiesScript.sml
@@ -3,6 +3,16 @@ open HolKernel Parse boolLib bossLib
 open grammarTheory
 open lcsymtacs
 open pred_setTheory
+open listTheory
+
+val rveq = rpt BasicProvers.VAR_EQ_TAC
+fun asm_match q = Q.MATCH_ASSUM_RENAME_TAC q []
+
+val MAP_EQ_CONS = prove(
+  ``(MAP f l = h::t) ⇔ ∃e es. l = e::es ∧ f e = h ∧ MAP f es = t``,
+  Cases_on `l` >> simp[])
+
+fun Store_thm(n,t,tac) = store_thm(n,t,tac) before export_rewrites [n]
 
 val _ = new_theory "NTproperties"
 
@@ -68,31 +78,6 @@ val nullable_NIL = store_thm(
   ``nullable G [] = T``,
   simp[nullable_def])
 val _ = export_rewrites ["nullable_NIL"]
-
-val derives_split_horizontally = store_thm(
-  "derives_split_horizontally",
-  ``∀p s sf. derives G (p ++ s) sf ⇔
-             ∃sf1 sf2. sf = sf1 ++ sf2 ∧ derives G p sf1 ∧ derives G s sf2``,
-  rpt gen_tac >> REVERSE eq_tac >- metis_tac [derives_paste_horizontally] >>
-  `∃sf0. p ++ s = sf0` by simp[] >> simp[] >>
-  pop_assum
-    (fn th => disch_then
-                (fn th2 => mp_tac th >> map_every qid_spec_tac [`s`, `p`] >>
-                           mp_tac th2)) >>
-  map_every qid_spec_tac [`sf`, `sf0`] >>
-  ho_match_mp_tac relationTheory.RTC_INDUCT >> simp[] >> conj_tac
-  >- metis_tac[relationTheory.RTC_REFL] >>
-  map_every qx_gen_tac [`sf0`, `sf'`, `sf`] >> simp[derive_def] >>
-  disch_then (CONJUNCTS_THEN2
-               (qxchl [`pfx`, `N`, `r`, `sfx`] strip_assume_tac)
-               strip_assume_tac) >> rw[] >>
-  qpat_assum `X = Y` mp_tac >> simp[listTheory.APPEND_EQ_APPEND_MID] >>
-  disch_then (DISJ_CASES_THEN (qxchl [`l`] strip_assume_tac)) >> rw[] >|[
-    first_x_assum (qspecl_then [`pfx ++ r ++ l`, `s`] mp_tac),
-    first_x_assum (qspecl_then [`p`, `l ++ r ++ sfx`] mp_tac)
-  ] >> simp[] >> disch_then (qxchl [`sf1`, `sf2`] strip_assume_tac) >> rw[] >>
-  map_every qexists_tac [`sf1`, `sf2`] >> simp[] >> match_mp_tac RTC_R_I >>
-  metis_tac[derive_def]);
 
 val nullable_CONS_NT = store_thm(
   "nullable_CONS_NT",
@@ -252,5 +237,295 @@ val nullableML_EQN = store_thm(
   ``nullable G sf ⇔ nullableML G ∅ sf``,
   metis_tac[nullable_nullableML, nullableML_nullable])
 
+(* ----------------------------------------------------------------------
+    Calculating first sets
+   ---------------------------------------------------------------------- *)
+
+val firstSet_def = Define`
+  firstSet G sf = { t | ∃rest. derives G sf (TOK t :: rest) }
+`;
+
+val firstSet_nonempty_fringe = store_thm(
+  "firstSet_nonempty_fringe",
+  ``∀pt t rest. ptree_fringe pt = TOK t :: rest ∧ valid_ptree G pt ⇒
+                t ∈ firstSet G [ptree_head pt]``,
+  simp[firstSet_def] >> metis_tac [grammarTheory.valid_ptree_derive]);
+
+val IN_firstSet = store_thm(
+  "IN_firstSet",
+  ``t ∈ firstSet G [sym] ⇒
+    ∃pt rest. ptree_head pt = sym ∧ valid_ptree G pt ∧
+              ptree_fringe pt = TOK t :: rest``,
+  simp[firstSet_def] >>
+  metis_tac [grammarTheory.ptrees_derive_extensible
+               |> Q.SPECL [`Lf sym`, `TOK t :: rest`]
+               |> SIMP_RULE (srw_ss()) []]);
+
+val derives_preserves_leading_toks = store_thm(
+  "derives_preserves_leading_toks",
+  ``∀G syms rest x.
+        derives G (MAP TOK syms ++ rest) x ⇔
+        ∃rest'. derives G rest rest' ∧ x = MAP TOK syms ++ rest'``,
+  rpt gen_tac >> eq_tac
+  >- (`∀x y. derives G x y ⇒
+             ∀syms rest.
+               (x = MAP TOK syms ++ rest) ⇒
+               ∃rest'. derives G rest rest' ∧ y = MAP TOK syms ++ rest'`
+        suffices_by metis_tac[] >>
+      ho_match_mp_tac relationTheory.RTC_INDUCT >> rw[] >>
+      fs[grammarTheory.derive_def] >> rveq >>
+      qpat_assum `MAP TOK syms ++ rest = Y` mp_tac >>
+      dsimp[listTheory.APPEND_EQ_APPEND, MAP_EQ_APPEND, MAP_EQ_CONS,
+            listTheory.APPEND_EQ_SING] >> rw[] >>
+      first_x_assum (qspec_then `syms` mp_tac) >>
+      simp_tac bool_ss [listTheory.APPEND_11, GSYM APPEND_ASSOC] >>
+      rw[] >>
+      metis_tac [grammarTheory.derive_def, relationTheory.RTC_CASES1,
+                 listTheory.APPEND]) >>
+  rw[] >> match_mp_tac grammarTheory.derives_paste_horizontally >>
+  simp[]);
+
+val firstSet_NIL = Store_thm(
+  "firstSet_NIL",
+  ``firstSet G [] = {}``,
+  simp[firstSet_def] >> simp[Once relationTheory.RTC_CASES1] >>
+  simp[grammarTheory.derive_def]);
+
+val firstSet_TOK = store_thm(
+  "firstSet_TOK",
+  ``firstSet G (TOK t::rest) = {t}``,
+  simp[firstSet_def, EXTENSION, EQ_IMP_THM] >> rw[]
+  >- (qspecl_then [`G`, `[t]`, `rest`] mp_tac derives_preserves_leading_toks >>
+      simp[] >> strip_tac >> fs[]) >>
+  metis_tac[relationTheory.RTC_REFL]);
+val _ = export_rewrites ["firstSet_TOK"]
+
+
+val firstSet_NT = store_thm(
+  "firstSet_NT",
+  ``firstSet G (NT N :: rest) =
+      if N ∈ FDOM G.rules then
+        BIGUNION (IMAGE (firstSet G) (G.rules ' N)) ∪
+        (if nullable G [NT N] then firstSet G rest
+         else {})
+      else {}``,
+  reverse (Cases_on `N ∈ FDOM G.rules`)
+  >- simp[firstSet_def, derives_leading_nonNT] >>
+  simp[Once EXTENSION] >> qx_gen_tac `t` >> reverse eq_tac
+  >- (dsimp[] >> rw[] >> fs[firstSet_def]
+      >- (asm_match `rhs ∈ G.rules ' N` >>
+          asm_match `derives G rhs (TOK t :: rest0)` >>
+          qexists_tac`rest0 ++ rest` >>
+          match_mp_tac RTC_R_I >>
+          qexists_tac `rhs ++ rest` >> simp[grammarTheory.derive_def] >>
+          metis_tac [listTheory.APPEND, APPEND_ASSOC,
+                     grammarTheory.derives_paste_horizontally,
+                     relationTheory.RTC_REFL]) >>
+      fs[nullable_def] >>
+      metis_tac [listTheory.APPEND,
+                 grammarTheory.derives_paste_horizontally]) >>
+  dsimp[firstSet_def] >> qx_gen_tac `rest'` >> strip_tac >>
+  `∃Z1 Z2. derives G [NT N] Z1 ∧ derives G rest Z2 ∧
+           (TOK t :: rest' = Z1 ++ Z2)`
+    by metis_tac [derives_split_horizontally, listTheory.APPEND] >>
+  Cases_on `Z1`
+  >- (`nullableNT G N` by fs[nullable_def] >> fs[] >> metis_tac[]) >>
+  fs[] >> rveq >>
+  qpat_assum `derives G [NT N] X`
+    (mp_tac o ONCE_REWRITE_RULE [relationTheory.RTC_CASES1]) >>
+  simp[] >> metis_tac[]);
+
+val firstSetML_def = tDefine "firstSetML" `
+  firstSetML seen [] = {} ∧
+  firstSetML seen (TOK t :: _) = {t} ∧
+  firstSetML seen (NT n :: rest) =
+    if n ∈ FDOM G.rules then
+      (if n ∉ seen then
+        BIGUNION (IMAGE (firstSetML (n INSERT seen))
+                        (G.rules ' n))
+       else {}) ∪
+      (if nullable G [NT n] then firstSetML seen rest
+       else {})
+    else {}
+`
+  (WF_REL_TAC `measure (λs. CARD (FDOM G.rules DIFF s)) LEX measure LENGTH` >>
+   simp[] >> rw[] >> DISJ1_TAC >> simp[CARD_DIFF_EQN] >>
+   simp[Once INTER_COMM] >> simp[INSERT_INTER] >>
+   simp[FINITE_INTER] >> simp[Once INTER_COMM] >>
+   simp[arithmeticTheory.SUB_LEFT_LESS] >>
+   match_mp_tac arithmeticTheory.LESS_LESS_EQ_TRANS >>
+   qexists_tac `CARD (n INSERT FDOM G.rules ∩ seen)` >>
+   conj_tac >- simp[] >>
+   `FINITE (FDOM G.rules)` by simp[] >>
+   pop_assum (MATCH_MP_TAC o MATCH_MP CARD_SUBSET) >>
+   simp[SUBSET_DEF])
+
+val firstSetML_firstSet = store_thm(
+  "firstSetML_firstSet",
+  ``∀seen sf. firstSetML G seen sf ⊆ firstSet G sf``,
+  ho_match_mp_tac (theorem "firstSetML_ind") >> simp[firstSetML_def] >>
+  map_every qx_gen_tac [`seen`, `N`, `sf`] >> strip_tac >>
+  reverse (Cases_on `N ∈ FDOM G.rules`) >> fs[] >>
+  reverse conj_tac
+  >- (rw[] >> fs[] >> simp[firstSet_NT] >> fs[SUBSET_DEF]) >>
+  Cases_on `N ∈ seen` >> simp[] >>
+  dsimp[SUBSET_DEF] >> simp[firstSet_NT] >> rpt strip_tac >>
+  DISJ1_TAC >> dsimp[] >> fs[SUBSET_DEF] >> metis_tac[]);
+
+val nts_derive_def = Define`
+  (nts_derive G [] tok ⇔ F) ∧
+  (nts_derive G [N] tok ⇔
+    N ∈ FDOM G.rules ∧
+    ∃p s. p ++ [TOK tok] ++ s ∈ G.rules ' N ∧
+          nullable G p) ∧
+  (nts_derive G (N1::N2::NS) tok ⇔
+    N1 ∈ FDOM G.rules ∧
+    ∃p s. p ++ [NT N2] ++ s ∈ G.rules ' N1 ∧
+          nullable G p ∧
+          nts_derive G (N2::NS) tok)
+`;
+val _ = export_rewrites ["nts_derive_def"]
+
+val nts_derive_APPEND_E = store_thm(
+  "nts_derive_APPEND_E",
+  ``nts_derive G (n1 ++ n2) t ∧ n2 ≠ [] ⇒ nts_derive G n2 t``,
+  Induct_on `n1` >> simp[] >> reverse (Cases_on `n1`)
+  >- (rpt strip_tac >> fs[]) >>
+  fs[] >> Cases_on `n2` >> simp[] >> metis_tac[]);
+
+val firstSetML_nullable_prefix = store_thm(
+  "firstSetML_nullable_prefix",
+  ``x ∈ firstSetML G sn sf ∧ nullable G p ⇒
+    x ∈ firstSetML G sn (p ++ sf)``,
+  Induct_on `p` >> simp[] >> Cases >>
+  simp[firstSetML_def, nullable_CONS_NT]);
+
+val firstSetML_CONS_I = store_thm(
+  "firstSetML_CONS_I",
+  ``tk ∈ firstSetML G sn [h] ⇒ tk ∈ firstSetML G sn (h::t)``,
+  Cases_on `h` >> simp[firstSetML_def] >> rw[]);
+
+val firstSet_CONS_I = store_thm(
+  "firstSet_CONS_I",
+  ``tk ∈ firstSet G [h] ⇒ tk ∈ firstSet G (h::t)``,
+  Cases_on `h` >> simp[firstSet_NT] >> rw[]);
+
+val distinct_nts_derive_firstSetML = store_thm(
+  "distinct_nts_derive_firstSetML",
+  ``∀sn. nts_derive G ns tok ∧ ALL_DISTINCT ns ∧
+         set ns ∩ sn = ∅ ⇒
+         tok ∈ firstSetML G sn [NT (HD ns)]``,
+  Induct_on `ns` >> simp[] >>
+  Cases_on `ns`
+  >- (simp[firstSetML_def] >> map_every qx_gen_tac [`N`, `seen`] >>
+      simp[Once EXTENSION] >> dsimp[] >>
+      map_every qx_gen_tac [`p`, `s`] >> strip_tac >>
+      qexists_tac `p ++ [TOK tok] ++ s` >> simp[] >>
+      REWRITE_TAC [GSYM APPEND_ASSOC] >>
+      match_mp_tac firstSetML_nullable_prefix >>
+      simp[firstSetML_def]) >>
+  simp[EXTENSION] >> rpt strip_tac >>
+  asm_match `p ++ [NT N'] ++ s ∈ G.rules ' N` >>
+  simp[firstSetML_def] >> `N ∉ sn` by metis_tac[] >>
+  dsimp[] >> qexists_tac `p ++ [NT N'] ++ s` >> simp[] >>
+  REWRITE_TAC [GSYM APPEND_ASSOC] >>
+  match_mp_tac firstSetML_nullable_prefix >> simp[] >>
+  match_mp_tac firstSetML_CONS_I >> fs[] >>
+  first_x_assum match_mp_tac >> simp[EXTENSION] >>
+  metis_tac[]);
+
+val heads_give_first = prove(
+  ``FLAT (MAP ptree_fringe subs) = tk :: rest ⇒
+    ∃p sym s r0.
+      p ++ [sym] ++ s = subs ∧ ptree_fringe sym = tk :: r0 ∧
+      FLAT (MAP ptree_fringe p) = []``,
+  Induct_on `subs` >> simp[] >> simp[APPEND_EQ_CONS] >> rpt strip_tac >>
+  dsimp[] >>fs[] >> map_every qexists_tac [`sym`, `s`, `r0`, `p`] >> simp[]);
+
+val nullable_alltrees = store_thm(
+  "nullable_alltrees",
+  ``nullable G sf ⇔
+    ∀sym. MEM sym sf ⇒
+          ∃pt. valid_ptree G pt ∧ ptree_head pt = sym ∧ ptree_fringe pt = []``,
+  simp[Once nullable_by_singletons] >> eq_tac >> rpt strip_tac >> res_tac
+  >- (pop_assum mp_tac >> simp_tac (srw_ss())[nullable_def] >>
+      simp[singleton_derives_ptree]) >>
+  simp[nullable_def] >> rw[] >> metis_tac [valid_ptree_derive]);
+
+val MEM_last_strip = prove(
+  ``∀l. MEM e l ⇒ ∃p s. l = p ++ [e] ++ s ∧ ¬MEM e s``,
+  ho_match_mp_tac rich_listTheory.SNOC_INDUCT >> dsimp[] >> conj_tac
+  >- (qx_gen_tac `l` >> strip_tac >> map_every qexists_tac [`l`, `[]`] >>
+      simp[]) >>
+  map_every qx_gen_tac [`l`, `x`] >> rpt strip_tac >> fs[] >>
+  Cases_on `x = e`
+  >- (map_every qexists_tac [`p ++ [e] ++ s`, `[]`] >> simp[]) >>
+  map_every qexists_tac [`p`, `s ++ [x]`] >> simp[]);
+
+val firstSet_nts_derive = store_thm(
+  "firstSet_nts_derive",
+  ``tk ∈ firstSet G [NT N] ⇒
+    ∃Ns. ALL_DISTINCT Ns ∧ nts_derive G Ns tk ∧ HD Ns = N``,
+  strip_tac >> pop_assum (strip_assume_tac o MATCH_MP IN_firstSet) >>
+  rpt (pop_assum mp_tac) >> map_every qid_spec_tac [`N`, `rest`, `pt`] >>
+  ho_match_mp_tac ptree_ind >> simp[] >> rpt strip_tac >>
+  imp_res_tac heads_give_first >> rveq >> fs[DISJ_IMP_THM, FORALL_AND_THM] >>
+  `nullable G (MAP ptree_head p)`
+    by (dsimp[nullable_alltrees, MEM_MAP] >>
+        full_simp_tac (srw_ss() ++ boolSimps.DNF_ss) [MEM_MAP, FLAT_EQ_NIL] >>
+        metis_tac[]) >>
+  Cases_on `ptree_head sym`
+  >- (qexists_tac `[s]` >> simp[] >> Cases_on `sym` >> fs[] >> metis_tac[]) >>
+  fs[] >> asm_match `nts_derive G Ns tk` >>
+  Cases_on `MEM s Ns`
+  >- (pop_assum (qxchl [`Ns0`, `Ns1`] strip_assume_tac o
+                 MATCH_MP MEM_last_strip) >>
+      `nts_derive G (s::Ns1) tk`
+        by (match_mp_tac (GEN_ALL nts_derive_APPEND_E) >> simp[] >>
+            fs[] >> qexists_tac `Ns0` >>
+            RULE_ASSUM_TAC (REWRITE_RULE[GSYM APPEND_ASSOC, APPEND]) >>
+            simp[]) >>
+      qexists_tac `s::Ns1` >> simp[] >> fs[ALL_DISTINCT_APPEND]) >>
+  qexists_tac `s::Ns` >> simp[] >> Cases_on `Ns` >> fs[] >> metis_tac[]);
+
+val firstSet_singleton = store_thm(
+  "firstSet_singleton",
+  ``tk ∈ firstSet G sf ⇔
+    ∃p e s. sf = p ++ [e] ++ s ∧ nullable G p ∧ tk ∈ firstSet G [e]``,
+  Induct_on `sf` >> simp[] >> Cases_on `h` >> simp[] >> eq_tac >> strip_tac
+  >- (map_every qexists_tac [`[]`, `TOK tk`, `sf`] >> simp[])
+  >- (fs[APPEND_EQ_CONS] >> rw[] >> fs[])
+  >- (fs[firstSet_NT] >> pop_assum mp_tac >> rw[]
+      >- (asm_match `rhs ∈ G.rules ' N` >>
+          map_every qexists_tac [`[]`, `NT N`, `sf`] >> simp[] >>
+          dsimp[firstSet_NT] >> metis_tac[])
+      >- (asm_match `nullableNT G N` >> asm_match `tk ∈ firstSet G [e]` >>
+          asm_match `nullable G p` >>
+          map_every qexists_tac [`NT N::p`, `e`] >> simp[] >>
+          simp[Once nullable_by_singletons, DISJ_IMP_THM, FORALL_AND_THM] >>
+          metis_tac[nullable_by_singletons]) >>
+      asm_match `tk ∈ firstSet G rhs` >> asm_match `rhs ∈ G.rules ' N` >>
+      map_every qexists_tac [`[]`, `NT N`, `sf`] >> simp[] >>
+      simp[firstSet_NT] >> metis_tac[]) >>
+  Cases_on `p` >> fs[] >> rw[] >- simp[firstSet_CONS_I] >>
+  fs[Once nullable_by_singletons, DISJ_IMP_THM, FORALL_AND_THM] >>
+  simp[firstSet_NT] >> fs[nullable_CONS_NT] >> metis_tac[]);
+
+val firstSet_firstSetML = store_thm(
+  "firstSet_firstSetML",
+  ``tk ∈ firstSet G sf ⇒ tk ∈ firstSetML G {} sf``,
+  simp[Once firstSet_singleton] >> rw[] >> REWRITE_TAC [GSYM APPEND_ASSOC] >>
+  match_mp_tac firstSetML_nullable_prefix >> simp[] >>
+  match_mp_tac firstSetML_CONS_I >>
+  asm_match `tk ∈ firstSet G [sym]` >>
+  Cases_on `sym` >> fs[] >- simp[firstSetML_def] >>
+  imp_res_tac firstSet_nts_derive >> rw[] >>
+  match_mp_tac distinct_nts_derive_firstSetML >> simp[]);
+
+val firstSetML_eqn = store_thm(
+  "firstSetML_eqn",
+  ``firstSet G sf = firstSetML G {} sf``,
+  simp[EXTENSION, EQ_IMP_THM, firstSet_firstSetML] >>
+  metis_tac [SUBSET_DEF, firstSetML_firstSet]);
 
 val _ = export_theory()
